Hoare/TerminationTriple.thy
@@ -17,13 +17,6 @@ lemma all_context_rest :
   (rest ** all_context) (contexts_as_set v2 c)"
   by (metis all_context_def context_maximal inf_bot_right sep_def set_pred.commute sup_bot.right_neutral)
 
-(*
-lemma gas_decreases_in_triples :
- "vctx_gas v2 \<ge> vctx_gas v1 \<Longrightarrow>
-  (all ** gas_pred g) (contexts_as_set v1 c) \<Longrightarrow>
-  (all ** gas_smaller g) (contexts_as_set v2 c)"
-*)
-
 definition all_with_gas :: "int \<Rightarrow> state_element set_pred" where
 "all_with_gas g s = (\<exists>c v.  s = contexts_as_set v c \<and>
    vctx_gas v = g \<and> vctx_memory_usage v \<ge> 0)"
@@ -103,18 +96,6 @@ lemma construct_perhaps_gas :
  (rest ** all_perhaps_less_gas g) (contexts_as_set v2 co_ctx)"
   by (metis all_perhaps_less_gas_def emp_def imp_sepL sep_emp set_pred.commute)
 
-lemma normal_case : assumes
- a:"(rest ** all_with_gas g) (contexts_as_set v1 co_ctx)" and
- b:"instruction_sem v1 co_ctx inst = InstructionContinue v2"
- shows  "(rest ** all_with_less_gas g) (contexts_as_set v2 co_ctx)"
-proof -
-  from a have "vctx_memory_usage v1 \<ge> 0 \<and> vctx_gas v1 = g"
-    using all_with_gas_gas all_with_gas_memu by auto
-  then have "vctx_memory_usage v2 \<ge> 0 \<and> vctx_gas v2 < g"
-   using b continue_decr_gas memu_good by fastforce
-  then show ?thesis using construct_less_gas all_with_gas_max a by fastforce
-qed
-
 lemma add_action :
 "rest (insert (ContinuingElm False)
      (contexts_as_set v2 co_ctx)) \<Longrightarrow>
@@ -126,6 +107,18 @@ apply (simp add: instruction_result_as_set_def
               action_def sep_def action_not_context)
 apply force
 done
+
+lemma normal_case : assumes
+ a:"(rest ** all_with_gas g) (contexts_as_set v1 co_ctx)" and
+ b:"instruction_sem v1 co_ctx inst = InstructionContinue v2"
+ shows  "(rest ** all_with_less_gas g) (contexts_as_set v2 co_ctx)"
+proof -
+  from a have "vctx_memory_usage v1 \<ge> 0 \<and> vctx_gas v1 = g"
+    using all_with_gas_gas all_with_gas_memu by auto
+  then have "vctx_memory_usage v2 \<ge> 0 \<and> vctx_gas v2 < g"
+   using b continue_decr_gas memu_good by fastforce
+  then show ?thesis using construct_less_gas all_with_gas_max a by fastforce
+qed
 
 lemma call_case : assumes
  a:"(rest ** all_with_gas g) (contexts_as_set v1 co_ctx)" and
@@ -212,7 +205,11 @@ proof -
   then have "(not_continuing ** rest ** all_perhaps_less_gas g)
     (insert (ContinuingElm False) (contexts_as_set v2 co_ctx))"
     by (simp add: not_continuing_sep)
-  then show ?thesis by (smt add_action failing_def)
+  then show ?thesis
+    using add_action
+      [of "not_continuing ** rest ** all_perhaps_less_gas g" v2 co_ctx
+        "\<lambda>y. \<exists>x. ContractFail x = y" "ContractFail x1" x33]
+    by (simp add: failing_def)
 qed
 
 lemma suicide_case : assumes
@@ -281,8 +278,7 @@ lemma using_gas_triple :
 apply(auto simp add: triple_def)
  apply(rule_tac x = 1 in exI)
  apply(case_tac presult; auto)
-apply (simp add:sep_add_def 
-  program_sem.simps next_state_def)
+apply (simp add:sep_add_def  program_sem.simps next_state_def)
 apply (case_tac "vctx_next_instruction x1 co_ctx")
 apply (auto simp add:case_1 meter_gas_check)
 apply (simp add: instruction_result_as_set_def)
@@ -321,5 +317,339 @@ using suicide_case apply force
 using return_case apply force
 done
 done
+
+(* need to start from beginning, more general or perhaps less
+   strict *)
+
+lemma perhaps_less :
+  "all_perhaps_less_gas g = all_with_less_gas (g+1)"
+apply (auto simp:all_perhaps_less_gas_def all_with_less_gas_def)
+done
+
+lemma case_2 :
+assumes a :
+ "(rest ** all_perhaps_less_gas g) (contexts_as_set x1 co_ctx)"
+shows  "(rest ** not_continuing ** all_perhaps_less_gas g ** failing)
+           (insert (ContinuingElm False)
+             (insert
+               (ContractActionElm (ContractFail lst))
+               (contexts_as_set x1 co_ctx)))"
+proof -
+  let ?set =  "contexts_as_set x1 co_ctx"
+  let ?base =  "rest ** all_perhaps_less_gas g"
+from a have "(?base ** not_continuing) (insert (ContinuingElm False) ?set)"
+  using context_cont1 not_cont_insert by presburger
+then have "(?base ** not_continuing)
+   (insert (ContinuingElm False) ?set-{ContractActionElm (ContractFail lst)})"
+  by (metis (full_types) Diff_empty Diff_insert2 context_cont context_cont1 contexts_as_set_def insert_minus state_element.distinct(685))
+then show ?thesis
+  by (metis failing_insert insert_commute sep_three set_pred.commute) 
+qed
+
+lemma perhaps_gas_max :
+   "(rest ** all_perhaps_less_gas g) (contexts_as_set v1 co_ctx) \<Longrightarrow>
+    rest {}"
+  by (smt all_perhaps_less_gas_def inf_sup_absorb maximality sep_def sup.cobounded2)
+
+lemma perhaps_gas_memu :
+   "(rest ** all_perhaps_less_gas g) (contexts_as_set v1 co_ctx) \<Longrightarrow>
+    vctx_memory_usage v1 \<ge> 0"
+  by (smt Un_upper2 all_perhaps_less_gas_def get_condition1 sep_def)
+
+lemma perhaps_gas_gas :
+   "(rest ** all_perhaps_less_gas g) (contexts_as_set v1 co_ctx) \<Longrightarrow>
+    vctx_gas v1 \<le> g"
+  by (smt Un_upper2 all_perhaps_less_gas_def get_condition1 sep_def)
+
+
+
+lemma normal_case2 : assumes
+ a:"(rest ** all_perhaps_less_gas g) (contexts_as_set v1 co_ctx)" and
+ b:"instruction_sem v1 co_ctx inst = InstructionContinue v2"
+ shows  "(rest ** all_with_less_gas g) (contexts_as_set v2 co_ctx)"
+proof -
+  from a have "vctx_memory_usage v1 \<ge> 0 \<and> vctx_gas v1 \<le> g"
+    using perhaps_gas_gas perhaps_gas_memu by auto
+  then have "vctx_memory_usage v2 \<ge> 0 \<and> vctx_gas v2 < g"
+   using b continue_decr_gas memu_good by fastforce
+  then show ?thesis
+   using construct_less_gas perhaps_gas_max a by fastforce
+qed
+
+lemma call_case2 : assumes
+ a:"(rest ** all_perhaps_less_gas g) (contexts_as_set v1 co_ctx)" and
+ b:"instruction_sem v1 co_ctx inst =
+    InstructionToEnvironment (ContractCall x1) v2 x33"
+ shows "(calling ** not_continuing **
+           rest ** all_with_less_gas g)
+           (instruction_result_as_set co_ctx
+             (InstructionToEnvironment
+               (ContractCall x1) v2 x33))"
+proof -
+  from a have "vctx_memory_usage v1 \<ge> 0 \<and> vctx_gas v1 \<le> g"
+    using perhaps_gas_gas perhaps_gas_memu by auto
+  then have "vctx_memory_usage v2 \<ge> 0 \<and> vctx_gas v2 < g"
+   using b call_decr_gas memu_good_env by fastforce
+  then have "(rest ** all_with_less_gas g) (contexts_as_set v2 co_ctx)"
+   using construct_less_gas perhaps_gas_max a by fastforce
+  then have "(not_continuing ** rest ** all_with_less_gas g)
+    (insert (ContinuingElm False) (contexts_as_set v2 co_ctx))"
+    by (simp add: not_continuing_sep)
+  then show ?thesis  by (smt add_action calling_def)
+qed
+
+lemma delegatecall_case2 : assumes
+ a:"(rest ** all_perhaps_less_gas g) (contexts_as_set v1 co_ctx)" and
+ b:"instruction_sem v1 co_ctx inst =
+    InstructionToEnvironment (ContractDelegateCall x1) v2 x33"
+ shows "(delegating ** not_continuing **
+           rest ** all_with_less_gas g)
+           (instruction_result_as_set co_ctx
+             (InstructionToEnvironment
+               (ContractDelegateCall x1) v2 x33))"
+proof -
+  from a have "vctx_memory_usage v1 \<ge> 0 \<and> vctx_gas v1 \<le> g"
+    using perhaps_gas_gas perhaps_gas_memu by auto
+  then have "vctx_memory_usage v2 \<ge> 0 \<and> vctx_gas v2 < g"
+   using b delegatecall_decr_gas memu_good_env by fastforce
+  then have "(rest ** all_with_less_gas g) (contexts_as_set v2 co_ctx)"
+   using construct_less_gas perhaps_gas_max a by fastforce
+  then have "(not_continuing ** rest ** all_with_less_gas g)
+    (insert (ContinuingElm False) (contexts_as_set v2 co_ctx))"
+    by (simp add: not_continuing_sep)
+  then show ?thesis by (smt add_action delegating_def)
+qed
+
+lemma create_case2 : assumes
+ a:"(rest ** all_perhaps_less_gas g) (contexts_as_set v1 co_ctx)" and
+ b:"instruction_sem v1 co_ctx inst =
+    InstructionToEnvironment (ContractCreate x1) v2 x33"
+ shows "(creating ** not_continuing **
+           rest ** all_with_less_gas g)
+           (instruction_result_as_set co_ctx
+             (InstructionToEnvironment
+               (ContractCreate x1) v2 x33))"
+proof -
+  from a have "vctx_memory_usage v1 \<ge> 0 \<and> vctx_gas v1 \<le> g"
+    using perhaps_gas_gas perhaps_gas_memu by auto
+  then have "vctx_memory_usage v2 \<ge> 0 \<and> vctx_gas v2 < g"
+   using b create_decr_gas memu_good_env by fastforce
+  then have "(rest ** all_with_less_gas g) (contexts_as_set v2 co_ctx)"
+   using construct_less_gas perhaps_gas_max a by fastforce
+  then have "(not_continuing ** rest ** all_with_less_gas g)
+    (insert (ContinuingElm False) (contexts_as_set v2 co_ctx))"
+    by (simp add: not_continuing_sep)
+  then show ?thesis by (smt add_action creating_def)
+qed
+
+lemma fail_case2 : assumes
+ a:"(rest ** all_perhaps_less_gas g) (contexts_as_set v1 co_ctx)" and
+ b:"instruction_sem v1 co_ctx inst =
+    InstructionToEnvironment (ContractFail x1) v2 x33"
+ shows "(failing ** not_continuing **
+           rest ** all_perhaps_less_gas g)
+           (instruction_result_as_set co_ctx
+             (InstructionToEnvironment
+               (ContractFail x1) v2 x33))"
+proof -
+  from a have "vctx_memory_usage v1 \<ge> 0 \<and> vctx_gas v1 \<le> g"
+    using perhaps_gas_gas perhaps_gas_memu by auto
+  then have "vctx_memory_usage v2 \<ge> 0 \<and> vctx_gas v2 \<le> g"
+   using b memu_good_env env_meter_gas meter_gas_ge_0 by smt
+  then have "(rest ** all_perhaps_less_gas g) (contexts_as_set v2 co_ctx)"
+   using construct_perhaps_gas perhaps_gas_max a by blast
+  then have "(not_continuing ** rest ** all_perhaps_less_gas g)
+    (insert (ContinuingElm False) (contexts_as_set v2 co_ctx))"
+    by (simp add: not_continuing_sep)
+  then show ?thesis
+    using add_action
+      [of "not_continuing ** rest ** all_perhaps_less_gas g" v2 co_ctx
+        "\<lambda>y. \<exists>x. ContractFail x = y" "ContractFail x1" x33]
+    by (simp add: failing_def)
+qed
+
+lemma suicide_case2 : assumes
+ a:"(rest ** all_perhaps_less_gas g) (contexts_as_set v1 co_ctx)" and
+ b:"instruction_sem v1 co_ctx inst =
+    InstructionToEnvironment (ContractSuicide x1) v2 x33"
+ shows "(destructing ** not_continuing **
+           rest ** all_perhaps_less_gas g)
+           (instruction_result_as_set co_ctx
+             (InstructionToEnvironment
+               (ContractSuicide x1) v2 x33))"
+proof -
+  from a have "vctx_memory_usage v1 \<ge> 0 \<and> vctx_gas v1 \<le> g"
+    using perhaps_gas_gas perhaps_gas_memu by auto
+  then have "vctx_memory_usage v2 \<ge> 0 \<and> vctx_gas v2 \<le> g"
+   using b memu_good_env env_meter_gas meter_gas_ge_0 by smt
+  then have "(rest ** all_perhaps_less_gas g) (contexts_as_set v2 co_ctx)"
+   using construct_perhaps_gas perhaps_gas_max a by blast
+  then have "(not_continuing ** rest ** all_perhaps_less_gas g)
+    (insert (ContinuingElm False) (contexts_as_set v2 co_ctx))"
+    by (simp add: not_continuing_sep)
+  then show ?thesis
+    using add_action
+      [of "not_continuing ** rest ** all_perhaps_less_gas g" v2 co_ctx
+        "\<lambda>y. \<exists>x. ContractSuicide x = y" "ContractSuicide x1" x33]
+    by (simp add: destructing_def)
+    
+qed
+
+lemma return_case2 : assumes
+ a:"(rest ** all_perhaps_less_gas g) (contexts_as_set v1 co_ctx)" and
+ b:"instruction_sem v1 co_ctx inst =
+    InstructionToEnvironment (ContractReturn x1) v2 x33"
+ shows "(returning ** not_continuing **
+           rest ** all_perhaps_less_gas g)
+           (instruction_result_as_set co_ctx
+             (InstructionToEnvironment
+               (ContractReturn x1) v2 x33))"
+proof -
+  from a have "vctx_memory_usage v1 \<ge> 0 \<and> vctx_gas v1 \<le> g"
+    using perhaps_gas_gas perhaps_gas_memu by auto
+  then have "vctx_memory_usage v2 \<ge> 0 \<and> vctx_gas v2 \<le> g"
+   using b memu_good_env env_meter_gas meter_gas_ge_0 by smt
+  then have "(rest ** all_perhaps_less_gas g) (contexts_as_set v2 co_ctx)"
+   using construct_perhaps_gas perhaps_gas_max a by blast
+  then have "(not_continuing ** rest ** all_perhaps_less_gas g)
+    (insert (ContinuingElm False) (contexts_as_set v2 co_ctx))"
+    by (simp add: not_continuing_sep)
+  then show ?thesis by (smt add_action returning_def)
+qed
+
+lemma using_gas_triple2 :
+   "triple {} (all_perhaps_less_gas g ** continuing) {}
+    (all_with_less_gas g ** continuing 
+    ## all_with_less_gas g ** not_continuing **
+      (delegating ## calling ## creating)
+    ## all_perhaps_less_gas g ** not_continuing **
+       (failing ## returning  ## destructing))"
+apply(auto simp add: triple_def)
+ apply(rule_tac x = 1 in exI)
+ apply(case_tac presult; auto)
+apply (simp add:sep_add_def  program_sem.simps next_state_def)
+apply (case_tac "vctx_next_instruction x1 co_ctx")
+apply (auto simp add:case_1 meter_gas_check)
+apply (simp add: instruction_result_as_set_def)
+using case_2 apply force
+defer
+defer
+apply (simp add: instruction_result_as_set_def)
+using case_2 apply force
+using meter_gas_check apply force
+using meter_gas_check apply force
+apply (simp add: instruction_result_as_set_def)
+using case_2 apply force
+subgoal for co_ctx rest v1 inst
+apply (case_tac "instruction_sem v1 co_ctx inst"; auto)
+apply (simp add: instruction_result_as_set_def)
+using no_annotation_inst apply simp
+apply (case_tac x31; auto simp:simple)
+using call_case2 apply force
+using delegatecall_case2 apply force
+using create_case2 apply force
+using fail_case2 apply force
+using suicide_case2 apply force
+using return_case2 apply force
+done
+subgoal for co_ctx rest v1 inst
+apply (case_tac "instruction_sem v1 co_ctx inst"; auto)
+apply (simp add: instruction_result_as_set_def)
+using normal_case2 apply simp
+using no_annotation_inst apply simp
+apply (case_tac x31; auto simp:simple)
+using call_case2 apply force
+using delegatecall_case2 apply force
+using create_case2 apply force
+using fail_case2 apply force
+using suicide_case2 apply force
+using return_case2 apply force
+done
+done
+
+(*
+lemma using_gas_triple3 :
+   "triple {} (all_perhaps_less_gas g ** \<langle>g > 0\<rangle> ** continuing) {}
+    (all_with_less_gas g  ** \<langle>g-1 > 0\<rangle> ** continuing 
+    ## all_with_less_gas g ** not_continuing **
+      (delegating ## calling ## creating)
+    ## all_perhaps_less_gas g ** not_continuing **
+       (failing ## returning  ## destructing))"
+apply(auto simp add: triple_def)
+ apply(rule_tac x = 1 in exI)
+ apply(case_tac presult; auto)
+apply (simp add:sep_add_def  program_sem.simps next_state_def)
+apply (case_tac "vctx_next_instruction x1 co_ctx")
+apply (auto simp add:case_1 meter_gas_check)
+apply (simp add: instruction_result_as_set_def)
+using case_2 apply force
+defer
+defer
+apply (simp add: instruction_result_as_set_def)
+using case_2 apply force
+using meter_gas_check apply force
+using meter_gas_check apply force
+apply (simp add: instruction_result_as_set_def)
+using case_2 apply force
+subgoal for co_ctx rest v1 inst
+apply (case_tac "instruction_sem v1 co_ctx inst"; auto)
+apply (simp add: instruction_result_as_set_def)
+using no_annotation_inst apply simp
+apply (case_tac x31; auto simp:simple)
+using call_case2 apply force
+using delegatecall_case2 apply force
+using create_case2 apply force
+using fail_case2 apply force
+using suicide_case2 apply force
+using return_case2 apply force
+done
+subgoal for co_ctx rest v1 inst
+apply (case_tac "instruction_sem v1 co_ctx inst"; auto)
+apply (simp add: instruction_result_as_set_def)
+using normal_case2 apply simp
+using no_annotation_inst apply simp
+apply (case_tac x31; auto simp:simple)
+using call_case2 apply force
+using delegatecall_case2 apply force
+using create_case2 apply force
+using fail_case2 apply force
+using suicide_case2 apply force
+using return_case2 apply force
+done
+done
+*)
+lemma test :
+  " all_perhaps_less_gas (if 0 \<le> g then g else 0) **
+       \<langle> 0 < (if 0 \<le> g then g else 0) \<rangle> =
+    all_perhaps_less_gas g ** \<langle> 0 < g \<rangle>"
+apply (cases "0 \<le> g")
+apply auto
+done
+
+lemma false_zero : "\<langle> False \<rangle> = zero"
+apply (auto simp:zero_def pure_def)
+done
+
+lemma termination_triple :
+   "\<exists>y. y < 0 \<and>
+    triple {} (all_perhaps_less_gas g ** continuing) {}
+    (all_perhaps_less_gas y ** continuing ##
+      (all_with_less_gas g ** not_continuing **
+      (delegating ## calling ## creating)
+    ## all_perhaps_less_gas g ** not_continuing **
+       (failing ## returning  ## destructing)))"
+apply (rule loop_triple_int [of "\<lambda>g. all_perhaps_less_gas g ** continuing"
+  "all_with_less_gas g ** not_continuing **
+      (delegating ## calling ## creating)
+    ## all_perhaps_less_gas g ** not_continuing **
+       (failing ## returning  ## destructing)" g])
+
+using loop_triple_int [of "\<lambda>g. all_perhaps_less_gas g ** continuing"
+  "all_with_less_gas g ** not_continuing **
+      (delegating ## calling ## creating)
+    ## all_perhaps_less_gas g ** not_continuing **
+       (failing ## returning  ## destructing)" g]
+apply (auto simp:test false_zero zero_mul zero_add)
+
 
 end
